Fix vcg and start using it + start cleanup of Primitives_IMP

Cook_Levin/IMP-_To_SAS+/IMP-_To_IMP--/Binary_Arithmetic_IMP.thy
@@ -1,5 +1,9 @@
-theory Binary_Arithmetic_IMP 
-  imports Primitives_IMP_Minus Binary_Arithmetic_Nat IMP_Minus.Com
+theory Binary_Arithmetic_IMP
+  imports
+    Primitives_IMP_Minus
+    Binary_Arithmetic_Nat
+    IMP_Minus.Com
+    Utilities
 begin
 
 unbundle IMP_Minus_Minus_Com.no_com_syntax
@@ -7,7 +11,7 @@ unbundle IMP_Minus_Minus_Com.no_com_syntax
 subsection \<open>N-th bit of Natural Number\<close>
 
 fun nth_bit_of_num_nat' :: "nat \<Rightarrow> nat \<Rightarrow> nat" where
-  "nth_bit_of_num_nat' x n  = (if x \<noteq> 0 then 
+  "nth_bit_of_num_nat' x n  = (if x \<noteq> 0 then
                               (if n \<noteq> 0 then
                                 nth_bit_of_num_nat' (tl_nat x) (n-1)
                                else
@@ -44,24 +48,28 @@ definition "nth_bit_of_num_state_upd s \<equiv>
         tl_ret_state = tl_imp tl_state;
         nth_bit_of_num_x' = tl_ret tl_ret_state;
         nth_bit_of_num_n' = nth_bit_of_num_n s - 1;
-        ret = \<lparr>nth_bit_of_num_x = nth_bit_of_num_x', nth_bit_of_num_n = nth_bit_of_num_n', nth_bit_of_num_ret = nth_bit_of_num_ret s\<rparr>
+        ret = \<lparr>nth_bit_of_num_x = nth_bit_of_num_x',
+               nth_bit_of_num_n = nth_bit_of_num_n',
+               nth_bit_of_num_ret = nth_bit_of_num_ret s\<rparr>
       in
         ret
 "
 
-definition 
+definition
   "nth_bit_of_num_imp_compute_loop_condition s \<equiv>
   (let
      AND_neq_zero_a' = nth_bit_of_num_x s;
      AND_neq_zero_b' = nth_bit_of_num_n s;
      AND_neq_zero_ret' = 0;
-     AND_neq_zero_state = \<lparr>AND_neq_zero_a = AND_neq_zero_a', AND_neq_zero_b = AND_neq_zero_b', AND_neq_zero_ret = AND_neq_zero_ret'\<rparr>;
+     AND_neq_zero_state = \<lparr>AND_neq_zero_a = AND_neq_zero_a',
+                           AND_neq_zero_b = AND_neq_zero_b',
+                           AND_neq_zero_ret = AND_neq_zero_ret'\<rparr>;
      AND_neq_zero_state_ret = AND_neq_zero_imp AND_neq_zero_state;
      condition = AND_neq_zero_ret (AND_neq_zero_state_ret)
   in
      condition)"
 
-definition 
+definition
   "nth_bit_of_num_imp_after_loop s \<equiv>
        (let
           hd_xs' = nth_bit_of_num_x s;
@@ -69,8 +77,8 @@ definition
           hd_state = \<lparr>hd_xs = hd_xs', hd_ret = hd_ret'\<rparr>;
           hd_state_ret = hd_imp hd_state;
           hd_x = hd_ret hd_state_ret;
-          nth_bit_of_num_ret' = 
-                           (if nth_bit_of_num_x s \<noteq> 0 then 
+          nth_bit_of_num_ret' =
+                           (if nth_bit_of_num_x s \<noteq> 0 then
                               ((if hd_x \<noteq> 0 then
                                    1 \<comment> \<open>x \<noteq> 0 \<and> n = 0 \<and> hd_nat x \<noteq> 0\<close>
                                  else
@@ -87,8 +95,14 @@ definition
           ret)"
 
 
+lemmas nth_bit_of_num_imp_subprogram_simps =
+  nth_bit_of_num_imp_after_loop_def
+  nth_bit_of_num_state_upd_def
+  nth_bit_of_num_imp_compute_loop_condition_def
+
+
 function nth_bit_of_num_imp:: "nth_bit_of_num_state \<Rightarrow> nth_bit_of_num_state" where
-  "nth_bit_of_num_imp s = 
+  "nth_bit_of_num_imp s =
   (
     (if nth_bit_of_num_imp_compute_loop_condition s \<noteq> 0 then \<comment> \<open>While xs \<noteq> 0\<close>
       (
@@ -106,32 +120,22 @@ function nth_bit_of_num_imp:: "nth_bit_of_num_state \<Rightarrow> nth_bit_of_num
       )
     )
 )"
-  by pat_completeness auto
+  by simp+
 termination
-  by (relation "measure (\<lambda>s. nth_bit_of_num_n s)")
-    (auto simp: nth_bit_of_num_imp_compute_loop_condition_def AND_neq_zero_imp_correct tl_imp_correct nth_bit_of_num_state_upd_def Let_def split: if_splits)
-
-lemmas nth_bit_of_num_imp_subprogram_simps = 
-  nth_bit_of_num_imp_after_loop_def nth_bit_of_num_state_upd_def
-  nth_bit_of_num_imp_compute_loop_condition_def 
+  by (relation "measure nth_bit_of_num_n")
+    (simp add: nth_bit_of_num_imp_subprogram_simps AND_neq_zero_imp_correct tl_imp_correct
+      Let_def split: if_splits)+
 
 declare nth_bit_of_num_imp.simps [simp del]
 
 lemma nth_bit_of_num_imp_correct:
-  "nth_bit_of_num_ret (nth_bit_of_num_imp s) = nth_bit_of_num_nat (nth_bit_of_num_x s) (nth_bit_of_num_n s)"
-proof (induction s rule: nth_bit_of_num_imp.induct)
-  case (1 s)
-  then show ?case
-    apply(subst nth_bit_of_num_imp.simps)
-    apply(subst nth_bit_of_num_nat.simps)
-    by (auto simp del: nth_bit_of_num_nat.simps
-        simp add: nth_bit_of_num_imp_after_loop_def 
-        nth_bit_of_num_imp_compute_loop_condition_def
-        tl_imp_correct hd_imp_correct AND_neq_zero_imp_correct
-        nth_bit_of_num_state_upd_def Let_def
-        split: if_splits)
-qed 
-
+  "nth_bit_of_num_ret (nth_bit_of_num_imp s) =
+    nth_bit_of_num_nat (nth_bit_of_num_x s) (nth_bit_of_num_n s)"
+  apply (induction s rule: nth_bit_of_num_imp.induct)
+  apply (subst nth_bit_of_num_imp.simps)
+  apply (subst nth_bit_of_num_nat.simps)
+  by (simp del: nth_bit_of_num_nat.simps add: nth_bit_of_num_imp_subprogram_simps tl_imp_correct
+      hd_imp_correct AND_neq_zero_imp_correct Let_def split: if_splits)
 
 definition "nth_bit_of_num_state_upd_time t s \<equiv>
       let
@@ -151,7 +155,7 @@ definition "nth_bit_of_num_state_upd_time t s \<equiv>
         ret
 "
 
-definition 
+definition
   "nth_bit_of_num_imp_compute_loop_condition_time t s \<equiv>
   (let
      AND_neq_zero_a' = nth_bit_of_num_x s;
@@ -160,7 +164,9 @@ definition
      t = t + 2;
      AND_neq_zero_ret' = 0;
      t = t + 2;
-     AND_neq_zero_state = \<lparr>AND_neq_zero_a = AND_neq_zero_a', AND_neq_zero_b = AND_neq_zero_b', AND_neq_zero_ret = AND_neq_zero_ret'\<rparr>;
+     AND_neq_zero_state = \<lparr>AND_neq_zero_a = AND_neq_zero_a',
+                           AND_neq_zero_b = AND_neq_zero_b',
+                           AND_neq_zero_ret = AND_neq_zero_ret'\<rparr>;
      AND_neq_zero_state_ret = AND_neq_zero_imp AND_neq_zero_state;
      t = t + AND_neq_zero_imp_time 0 AND_neq_zero_state;
      condition = AND_neq_zero_ret AND_neq_zero_state_ret;
@@ -169,7 +175,7 @@ definition
   in
      t)"
 
-definition 
+definition
   "nth_bit_of_num_imp_after_loop_time t s \<equiv>
        (let
           hd_xs' = nth_bit_of_num_x s;
@@ -181,8 +187,8 @@ definition
           t = t + hd_imp_time 0 hd_state;
           hd_x = hd_ret hd_state_ret;
           t = t + 2;
-          nth_bit_of_num_ret'::nat = 
-                           (if nth_bit_of_num_x s \<noteq> 0 then 
+          nth_bit_of_num_ret'::nat =
+                           (if nth_bit_of_num_x s \<noteq> 0 then
                               ((if hd_x \<noteq> 0 then
                                    1 \<comment> \<open>x \<noteq> 0 \<and> n = 0 \<and> hd_nat x \<noteq> 0\<close>
                                  else
@@ -194,14 +200,14 @@ definition
                                  1 \<comment> \<open>x = 0 \<and> n = 0\<close>)
                               );
           t = t + 1 +
-                           (if nth_bit_of_num_x s \<noteq> 0 then 
+                           (if nth_bit_of_num_x s \<noteq> 0 then
                               (1 +
                                (if hd_x \<noteq> 0 then
                                   2 \<comment> \<open>x \<noteq> 0 \<and> n = 0 \<and> hd_nat x \<noteq> 0\<close>
                                 else
                                   2 \<comment> \<open>x \<noteq> 0 \<and> n = 0 \<and> hd_nat x = 0\<close>))
                             else
-                              1 + 
+                              1 +
                               (if nth_bit_of_num_n s \<noteq> 0 then
                                  2 \<comment> \<open>x = 0 \<and> n \<noteq> 0\<close>
                                else
@@ -212,17 +218,21 @@ definition
           ret
 )"
 
+lemmas nth_bit_of_num_imp_subprogram_time_simps =
+  nth_bit_of_num_imp_subprogram_simps
+  nth_bit_of_num_imp_after_loop_time_def nth_bit_of_num_state_upd_time_def
+  nth_bit_of_num_imp_compute_loop_condition_time_def
 
 function nth_bit_of_num_imp_time:: "nat \<Rightarrow> nth_bit_of_num_state \<Rightarrow> nat" where
-  "nth_bit_of_num_imp_time t s = 
+  "nth_bit_of_num_imp_time t s =
   nth_bit_of_num_imp_compute_loop_condition_time 0 s+
    (
     (if nth_bit_of_num_imp_compute_loop_condition s \<noteq> 0 then \<comment> \<open>While xs \<noteq> 0\<close>
       (
         let
           t = t + 1; \<comment> \<open>While condition true\<close>
-          next_iteration = 
-           nth_bit_of_num_imp_time (t + 
+          next_iteration =
+           nth_bit_of_num_imp_time (t +
                                     nth_bit_of_num_state_upd_time 0 s) (nth_bit_of_num_state_upd s)
         in
           next_iteration
@@ -239,42 +249,34 @@ function nth_bit_of_num_imp_time:: "nat \<Rightarrow> nth_bit_of_num_state \<Rig
 )"
   by pat_completeness auto
 termination
-  by (relation "measure (\<lambda>(t, s). nth_bit_of_num_n s)")
-    (auto simp: nth_bit_of_num_imp_compute_loop_condition_def
-      AND_neq_zero_imp_correct tl_imp_correct
-      nth_bit_of_num_state_upd_def Let_def
-      split: if_splits)
+  by (relation "measure (nth_bit_of_num_n \<circ> snd)")
+    (simp add: nth_bit_of_num_imp_subprogram_time_simps AND_neq_zero_imp_correct tl_imp_correct
+      Let_def split: if_splits)+
 
+declare nth_bit_of_num_imp_time.simps [simp del]
 
-lemmas nth_bit_of_num_imp_subprogram_time_simps = nth_bit_of_num_imp_subprogram_simps
-  nth_bit_of_num_imp_after_loop_time_def nth_bit_of_num_state_upd_time_def
-  nth_bit_of_num_imp_compute_loop_condition_time_def 
+lemma nth_bit_of_num_imp_time_acc: "(nth_bit_of_num_imp_time (Suc t) s) =
+  Suc (nth_bit_of_num_imp_time t s)"
+  by (induction t s rule: nth_bit_of_num_imp_time.induct)
+    ((subst (1 2) nth_bit_of_num_imp_time.simps);
+      (simp add: nth_bit_of_num_state_upd_def))
 
+lemma nth_bit_of_num_imp_time_acc_2_aux:
+  "(nth_bit_of_num_imp_time t s) =
+    t + (nth_bit_of_num_imp_time 0 s)"
+  by (induction t arbitrary: s)
+    (simp add: nth_bit_of_num_imp_time_acc)+
 
-lemmas [simp del] = nth_bit_of_num_imp_time.simps
+lemma nth_bit_of_num_imp_time_acc_2:
+  "t \<noteq> 0 \<Longrightarrow> (nth_bit_of_num_imp_time t s) =
+    t + (nth_bit_of_num_imp_time 0 s)"
+  by (rule nth_bit_of_num_imp_time_acc_2_aux)
 
-lemma nth_bit_of_num_imp_time_acc: "(nth_bit_of_num_imp_time (Suc t) s) = Suc (nth_bit_of_num_imp_time t s)"
-  apply (induction t s arbitrary:  rule: nth_bit_of_num_imp_time.induct)
-  apply(subst nth_bit_of_num_imp_time.simps)
-  apply(subst (2) nth_bit_of_num_imp_time.simps)
-  apply (auto simp add: nth_bit_of_num_imp_compute_loop_condition_time_def
-      nth_bit_of_num_imp_after_loop_time_def
-      nth_bit_of_num_state_upd_time_def
-      nth_bit_of_num_state_upd_def Let_def eval_nat_numeral 
-      split: if_splits)
-  done
-
-lemma nth_bit_of_num_imp_time_acc_2: "(nth_bit_of_num_imp_time x s) = x + (nth_bit_of_num_imp_time 0 s)"
-  by (induction x arbitrary: s)
-    (auto simp add: nth_bit_of_num_imp_time_acc nth_bit_of_num_state_upd_def Let_def eval_nat_numeral split: if_splits)
-
-lemma nth_bit_of_num_imp_time_acc_2_simp: 
-  "(nth_bit_of_num_imp_time (nth_bit_of_num_state_upd_time 0 s) s') =
-   (nth_bit_of_num_state_upd_time 0 s) + (nth_bit_of_num_imp_time 0 s')"
-  by (rule nth_bit_of_num_imp_time_acc_2)
-
-\<comment> \<open>The following separation is due to parsing time, whic grows exponentially in the length of IMP-
-    programs.\<close>
+lemma nth_bit_of_num_imp_time_acc_3:
+  "(nth_bit_of_num_imp_time (a + b) s) =
+    a + (nth_bit_of_num_imp_time b s)"
+  by (induction a arbitrary: b s)
+    (simp add: nth_bit_of_num_imp_time_acc)+
 
 abbreviation "nth_bit_of_num_while_cond \<equiv> ''condition''"
 
@@ -369,176 +371,70 @@ definition nth_bit_of_num_IMP_Minus where
     \<comment> \<open>)\<close>
 "
 
-abbreviation 
+abbreviation
   "nth_bit_of_num_IMP_vars \<equiv>
   {nth_bit_of_num_x_str, nth_bit_of_num_n_str, nth_bit_of_num_ret_str}"
 
-lemmas nth_bit_of_num_IMP_subprogram_simps = 
-  nth_bit_of_num_IMP_init_while_cond_def nth_bit_of_num_IMP_loop_body_def nth_bit_of_num_IMP_after_loop_def
+lemmas nth_bit_of_num_IMP_subprogram_simps =
+  nth_bit_of_num_IMP_init_while_cond_def
+  nth_bit_of_num_IMP_loop_body_def
+  nth_bit_of_num_IMP_after_loop_def
 
 definition "nth_bit_of_num_imp_to_HOL_state p s =
-  \<lparr>nth_bit_of_num_x = (s (add_prefix p nth_bit_of_num_x_str)), 
+  \<lparr>nth_bit_of_num_x = (s (add_prefix p nth_bit_of_num_x_str)),
    nth_bit_of_num_n = (s (add_prefix p nth_bit_of_num_n_str)),
    nth_bit_of_num_ret = (s (add_prefix p nth_bit_of_num_ret_str))\<rparr>"
 
-lemmas nth_bit_of_num_state_translators = tl_imp_to_HOL_state_def hd_imp_to_HOL_state_def
+lemmas nth_bit_of_num_state_translators =
+  tl_imp_to_HOL_state_def
+  hd_imp_to_HOL_state_def
   AND_neq_zero_imp_to_HOL_state_def
   nth_bit_of_num_imp_to_HOL_state_def
 
 lemmas nth_bit_of_num_complete_simps =
-  nth_bit_of_num_IMP_subprogram_simps nth_bit_of_num_imp_subprogram_simps
+  nth_bit_of_num_IMP_subprogram_simps
+  nth_bit_of_num_imp_subprogram_simps
   nth_bit_of_num_state_translators
 
-lemmas functional_correctness_lemmas = functional_correctness
-
-definition "While' = Com.com.While"
-
-notation While' ("(WHILEdummy _/\<noteq>0 DO _)"  [0, 61] 61)
-
-lemma While_tE_dummy:
-"(WHILE b\<noteq>0 DO c, s) \<Rightarrow>\<^bsup> x \<^esup> t \<Longrightarrow>
-(x = Suc (Suc 0) \<Longrightarrow> t = s \<Longrightarrow> s b = 0 \<Longrightarrow> P) \<Longrightarrow>
-(\<And>x' s2 y. 0 < s b \<Longrightarrow> (c, s) \<Rightarrow>\<^bsup> x' \<^esup> s2 \<Longrightarrow> (WHILEdummy b\<noteq>0 DO c, s2) \<Rightarrow>\<^bsup> y \<^esup> t \<Longrightarrow> Suc (x' + y) = x \<Longrightarrow> P) \<Longrightarrow> P"
-  by (auto simp: While'_def)
-
-method while_step = (erule While_tE_dummy, print_fact While_tE)
-method seq_step = (erule Seq_tE, print_fact Seq_tE)
-method if_step = (erule If_tE, print_fact If_tE)
-method assign_step = (drule AssignD, elim conjE, print_fact AssignD)
-
-definition "dest_com_gen = 0"
-
-lemma dest_com_gen: "dest_com_gen = dest_com_gen"
-  by auto
-
-method subroutine_step for vars::"char list set" =
-  (erule functional_correctness_lemmas[where vars = vars],
-     (match premises
-        in prem[thin]:
-          "_ \<in> vars" \<Rightarrow>
-                      \<open>match premises
-                          in c[thin]: "_" (multi) \<Rightarrow>
-                              \<open>insert prem, (auto)[1]\<close>\<close>))
-
-definition "subroutine_step = 0"
-
-lemma subroutine_step: "subroutine_step = subroutine_step"
-  by auto
-
-method dest_com_gen' = 
-  (erule compose_programs_1[where ?c2.0 = "(While' _ _)"], assumption,
-    erule compose_programs_2[where ?c1.0 = "(_;; While' _ _)"], assumption,
-    (match premises
-      in a[thin]: 
-      "(init_while_cond;; 
-                WHILEdummy _ \<noteq>0 DO (loop_body;; init_while_cond);;
-                after_loop, _) \<Rightarrow>\<^bsup>_\<^esup> _"
-    for init_while_cond loop_body after_loop  \<Rightarrow> 
-      \<open>match premises in b[thin]: "\<lbrakk>loop_cond; state_upd; _\<rbrakk> \<Longrightarrow> P"
-       for loop_cond state_upd P \<Rightarrow> \<open>subst b[OF _ _ a[unfolded While'_def]]\<close>\<close>))
-
-method vcg for vars::"char list set" = (*subroutine_step vars*)
-  (((subroutine_step vars, print_fact subroutine_step); (vcg vars)?) | (while_step ; (vcg vars)?) | ((dest_com_gen', print_fact dest_com_gen) ; (vcg vars)?) | (if_step ; (vcg vars)?) | (seq_step ; (vcg vars)?) | (assign_step; (vcg vars)?))
-
-lemma nth_bit_of_num_IMP_Minus_correct_function: 
+lemma nth_bit_of_num_IMP_Minus_correct_function:
   "(invoke_subprogram p nth_bit_of_num_IMP_Minus, s) \<Rightarrow>\<^bsup>t\<^esup> s' \<Longrightarrow>
-     s' (add_prefix p nth_bit_of_num_ret_str) = nth_bit_of_num_ret (nth_bit_of_num_imp (nth_bit_of_num_imp_to_HOL_state p s))"
-  apply(induction "nth_bit_of_num_imp_to_HOL_state p s" arbitrary: s s' t rule: nth_bit_of_num_imp.induct)
+    s' (add_prefix p nth_bit_of_num_ret_str) =
+      nth_bit_of_num_ret (nth_bit_of_num_imp (nth_bit_of_num_imp_to_HOL_state p s))"
+  apply(induction "nth_bit_of_num_imp_to_HOL_state p s" arbitrary: s s' t
+      rule: nth_bit_of_num_imp.induct)
   apply(subst nth_bit_of_num_imp.simps)
   apply(simp only: nth_bit_of_num_IMP_Minus_def prefix_simps)
   apply(vcg nth_bit_of_num_IMP_vars)
-   apply(simp only: nth_bit_of_num_IMP_subprogram_simps prefix_simps)
-  apply(vcg nth_bit_of_num_IMP_vars)
 
-   apply(simp add: nth_bit_of_num_imp_subprogram_simps nth_bit_of_num_imp_time_acc
-      nth_bit_of_num_state_translators Let_def,
-      force)
-     apply(simp add: nth_bit_of_num_imp_subprogram_simps nth_bit_of_num_imp_time_acc
-      nth_bit_of_num_state_translators Let_def,
-      force)
-     apply(simp add: nth_bit_of_num_imp_subprogram_simps nth_bit_of_num_imp_time_acc
-      nth_bit_of_num_state_translators Let_def,
-      force)
-     apply(simp add: nth_bit_of_num_imp_subprogram_simps nth_bit_of_num_imp_time_acc
-      nth_bit_of_num_state_translators Let_def,
-      force)
-
-   apply(simp_all only: nth_bit_of_num_IMP_init_while_cond_def nth_bit_of_num_IMP_loop_body_def prefix_simps)
-
+  subgoal
+    apply(subst (asm) (3) nth_bit_of_num_IMP_init_while_cond_def)
+    apply(subst (asm) (2) nth_bit_of_num_IMP_after_loop_def)
+    apply(simp only: prefix_simps)
     apply(vcg nth_bit_of_num_IMP_vars)
-   apply(simp only: nth_bit_of_num_imp_subprogram_simps nth_bit_of_num_imp_time_acc
-      nth_bit_of_num_state_translators Let_def;
-      force)
+    by (fastforce simp: nth_bit_of_num_complete_simps)+
 
-  apply(vcg nth_bit_of_num_IMP_vars)
-   apply(simp only: nth_bit_of_num_imp_subprogram_simps nth_bit_of_num_imp_time_acc
-      nth_bit_of_num_state_translators Let_def;
-      force)
-
+  subgoal
+    apply(subst (asm) (1) nth_bit_of_num_IMP_init_while_cond_def)
+    apply(simp only: prefix_simps)
     apply(vcg nth_bit_of_num_IMP_vars)
-   apply(simp only: nth_bit_of_num_imp_subprogram_simps nth_bit_of_num_imp_time_acc
-      nth_bit_of_num_state_translators Let_def;
-      force)
+    by (fastforce_sorted_premises simp: nth_bit_of_num_complete_simps)
+
+  subgoal
+    apply(subst (asm) nth_bit_of_num_IMP_init_while_cond_def)
+    apply(subst (asm) nth_bit_of_num_IMP_loop_body_def)
+    apply(simp only: prefix_simps)
+    apply(vcg nth_bit_of_num_IMP_vars)
+    by (fastforce_sorted_premises simp: Let_def
+        nth_bit_of_num_complete_simps)
+
+  subgoal
+    apply(subst (asm) (1) nth_bit_of_num_IMP_init_while_cond_def)
+    apply(subst (asm) (1) nth_bit_of_num_IMP_loop_body_def)
+    apply(simp only: prefix_simps)
+    apply(vcg nth_bit_of_num_IMP_vars)
+    by (fastforce_sorted_premises simp: Let_def
+        nth_bit_of_num_complete_simps)
   done
-
-(*lemma nth_bit_of_num_IMP_Minus_correct_function:
-  "(invoke_subprogram p nth_bit_of_num_IMP_Minus, s) \<Rightarrow>\<^bsup>t\<^esup> s' \<Longrightarrow>
-     s' (add_prefix p nth_bit_of_num_ret_str) = nth_bit_of_num_ret (nth_bit_of_num_imp (nth_bit_of_num_imp_to_HOL_state p s))"
-  apply(induction "nth_bit_of_num_imp_to_HOL_state p s" arbitrary: s s' t rule: nth_bit_of_num_imp.induct)
-  apply(subst nth_bit_of_num_imp.simps)
-  apply(simp only: nth_bit_of_num_IMP_Minus_def prefix_simps)
-  apply(erule Seq_tE)+
-  apply(erule While_tE)
-   apply(simp only: nth_bit_of_num_IMP_subprogram_simps prefix_simps)
-   apply(erule Seq_tE)+
-   apply(erule AND_neq_zero_IMP_Minus_correct[where vars = "nth_bit_of_num_IMP_vars"])
-    apply auto [1]
-   apply(erule If_tE)
-    apply(erule If_tE)
-     apply(drule AssignD)+
-     apply(elim conjE)
-     apply(erule hd_IMP_Minus_correct[where vars = "nth_bit_of_num_IMP_vars"])
-      apply auto [1]
-     apply(simp add: nth_bit_of_num_imp_subprogram_simps nth_bit_of_num_imp_time_acc
-      nth_bit_of_num_state_translators Let_def,
-      force)
-    apply(erule hd_IMP_Minus_correct[where vars = "nth_bit_of_num_IMP_vars"])
-     apply auto [1]
-    apply(simp add: nth_bit_of_num_imp_subprogram_simps nth_bit_of_num_imp_time_acc
-      nth_bit_of_num_state_translators Let_def,
-      force)
-   apply(erule hd_IMP_Minus_correct[where vars = "nth_bit_of_num_IMP_vars"])
-    apply auto [1]
-   apply(simp add: nth_bit_of_num_imp_subprogram_simps nth_bit_of_num_imp_time_acc
-      nth_bit_of_num_state_translators Let_def,
-      force)
-
-  apply(erule Seq_tE)+
-  apply(dest_com_gen)
-    apply(simp only: nth_bit_of_num_IMP_init_while_cond_def prefix_simps)
-    apply(erule Seq_tE)+
-    apply(erule AND_neq_zero_IMP_Minus_correct[where vars = "nth_bit_of_num_IMP_vars"])
-     apply auto [1]
-    apply(simp add: nth_bit_of_num_complete_simps Let_def, force)
-
-   apply(simp only: nth_bit_of_num_IMP_init_while_cond_def nth_bit_of_num_IMP_loop_body_def prefix_simps)
-   apply(erule Seq_tE)+
-   apply(erule AND_neq_zero_IMP_Minus_correct[where vars = "nth_bit_of_num_IMP_vars"])
-    apply auto [1]
-   apply(erule tl_IMP_Minus_correct[where vars = "nth_bit_of_num_IMP_vars"])
-    apply force [1]
-   apply(simp add: nth_bit_of_num_complete_simps Let_def, force)
-
-  apply(simp only: nth_bit_of_num_IMP_init_while_cond_def nth_bit_of_num_IMP_loop_body_def prefix_simps)
-  apply(erule Seq_tE)+
-  apply(erule AND_neq_zero_IMP_Minus_correct[where vars = "nth_bit_of_num_IMP_vars"])
-   apply auto [1]
-  apply(erule tl_IMP_Minus_correct[where vars = "nth_bit_of_num_IMP_vars"])
-   apply force [1]
-  apply(simp add: nth_bit_of_num_complete_simps Let_def, force)
-  done*)
-
-
 
 text \<open>Debugging lemma\<close>
 
@@ -558,80 +454,53 @@ lemma nth_bit_of_num_IMP_Minus_correct_time_loop_condition:
 
 lemmas nth_bit_of_num_complete_time_simps =
   nth_bit_of_num_imp_subprogram_time_simps
-  nth_bit_of_num_imp_time_acc
-  nth_bit_of_num_imp_time_acc_2_simp
-
-lemma While_tE_time_dummy:
-"(WHILE b\<noteq>0 DO c, s) \<Rightarrow>\<^bsup> x \<^esup> t \<Longrightarrow>
-  (x = Suc (Suc 0) \<Longrightarrow> t = s \<Longrightarrow> s b = 0 \<Longrightarrow> P) \<Longrightarrow>
-  (\<And>x' s2 y. 0 < s b \<Longrightarrow> (c, s) \<Rightarrow>\<^bsup> x' \<^esup> s2 \<Longrightarrow> (WHILEdummy b\<noteq>0 DO c, s2) \<Rightarrow>\<^bsup> y \<^esup> t \<Longrightarrow> x = Suc (x' + y) \<Longrightarrow> P) \<Longrightarrow> P"
-  by (auto simp: While'_def)
-
-method while_step_time = (erule While_tE_time_dummy, print_fact While_tE)
-
-method dest_com_gen_time' = 
-  (erule compose_programs_1[where ?c2.0 = "(While' _ _)"], assumption,
-    erule compose_programs_2[where ?c1.0 = "(_;; While' _ _)"], assumption,
-    (match premises
-      in a[thin]: 
-      "(init_while_cond;; 
-                WHILEdummy _ \<noteq>0 DO (loop_body;; init_while_cond);;
-                after_loop, _) \<Rightarrow>\<^bsup>_\<^esup> _"
-    for init_while_cond loop_body after_loop  \<Rightarrow> 
-      \<open>match premises in b[thin]: "\<lbrakk>loop_cond; state_upd; _\<rbrakk> \<Longrightarrow> P"
-       for loop_cond state_upd P \<Rightarrow> \<open>subst b[OF _ _ a[unfolded While'_def], simplified add.assoc]\<close>\<close>))
-
-
-method vcg_time for vars::"char list set" = (*subroutine_step vars*)
-  ((subroutine_step vars, print_fact subroutine_step) |
-   while_step_time | (dest_com_gen_time', print_fact dest_com_gen) | if_step | seq_step | assign_step)
-
+  nth_bit_of_num_imp_time_acc_2
+  nth_bit_of_num_imp_time_acc_3
+  nth_bit_of_num_state_translators
 
 lemma nth_bit_of_num_IMP_Minus_correct_time:
   "(invoke_subprogram p nth_bit_of_num_IMP_Minus, s) \<Rightarrow>\<^bsup>t\<^esup> s' \<Longrightarrow>
      t = nth_bit_of_num_imp_time 0 (nth_bit_of_num_imp_to_HOL_state p s)"
-  apply(induction "nth_bit_of_num_imp_to_HOL_state p s" arbitrary: s s' t rule: nth_bit_of_num_imp.induct)
+  apply(induction "nth_bit_of_num_imp_to_HOL_state p s"
+      arbitrary: s s' t rule: nth_bit_of_num_imp.induct)
   apply(subst nth_bit_of_num_imp_time.simps)
   apply(simp only: nth_bit_of_num_IMP_Minus_def prefix_simps)
-  apply(vcg_time nth_bit_of_num_IMP_vars)+
-   apply(simp only: nth_bit_of_num_IMP_subprogram_simps prefix_simps)
-  apply(vcg_time nth_bit_of_num_IMP_vars)+
-     apply(simp add: nth_bit_of_num_imp_subprogram_time_simps nth_bit_of_num_imp_time_acc
-      nth_bit_of_num_state_translators Let_def,
-      force)
-  apply(vcg_time nth_bit_of_num_IMP_vars)+
-     apply(simp add: nth_bit_of_num_imp_subprogram_time_simps nth_bit_of_num_imp_time_acc
-      nth_bit_of_num_state_translators Let_def,
-      force)
-  apply(vcg_time nth_bit_of_num_IMP_vars)+
-     apply(simp add: nth_bit_of_num_imp_subprogram_time_simps nth_bit_of_num_imp_time_acc
-      nth_bit_of_num_state_translators Let_def,
-      force)
-  apply(vcg_time nth_bit_of_num_IMP_vars)+
-     apply(simp add: nth_bit_of_num_imp_subprogram_time_simps nth_bit_of_num_imp_time_acc
-      nth_bit_of_num_state_translators Let_def,
-      force)
 
-  apply(vcg_time nth_bit_of_num_IMP_vars)+
+  apply(vcg_time nth_bit_of_num_IMP_vars)
+
+  subgoal
+    apply(subst (asm) (3) nth_bit_of_num_IMP_init_while_cond_def)
+    apply(subst (asm) (2) nth_bit_of_num_IMP_after_loop_def)
+    apply(simp only: prefix_simps)
+    apply(vcg_time nth_bit_of_num_IMP_vars)
+    by (force simp: nth_bit_of_num_IMP_subprogram_simps
+        nth_bit_of_num_imp_subprogram_time_simps
+        nth_bit_of_num_state_translators)+
+
   apply(simp add: add.assoc)
+  apply(vcg_time nth_bit_of_num_IMP_vars)
 
-    apply(simp only: nth_bit_of_num_IMP_init_while_cond_def prefix_simps)
-  apply(vcg_time nth_bit_of_num_IMP_vars)+
-    apply(simp add: nth_bit_of_num_complete_simps Let_def; force)
+  subgoal
+    apply(subst (asm) (1) nth_bit_of_num_IMP_init_while_cond_def)
+    apply(simp only: prefix_simps)
+    apply(vcg_time nth_bit_of_num_IMP_vars)
+    by (fastforce simp add: nth_bit_of_num_complete_simps)
 
-   apply(simp only: nth_bit_of_num_IMP_init_while_cond_def nth_bit_of_num_IMP_loop_body_def prefix_simps)
-  apply(vcg_time nth_bit_of_num_IMP_vars)+
-   apply(simp add: nth_bit_of_num_complete_simps Let_def; force)
+  subgoal
+    apply(subst (asm) (1) nth_bit_of_num_IMP_init_while_cond_def)
+    apply(subst (asm) (1) nth_bit_of_num_IMP_loop_body_def)
+    apply(simp only: prefix_simps)
+    apply(vcg_time nth_bit_of_num_IMP_vars)
+    by (fastforce_sorted_premises simp: Let_def
+        nth_bit_of_num_complete_time_simps)
 
-  apply(simp only: nth_bit_of_num_IMP_init_while_cond_def nth_bit_of_num_IMP_loop_body_def prefix_simps)
-  apply(vcg_time nth_bit_of_num_IMP_vars)+
-  apply(simp add: nth_bit_of_num_imp_time_acc_2[where x = "tl_imp_time t s" for t s]
-      nth_bit_of_num_complete_time_simps nth_bit_of_num_complete_simps Let_def;
-      force)
+  subgoal
+    apply(subst (asm) (1) nth_bit_of_num_IMP_init_while_cond_def)
+    apply(subst (asm) (1) nth_bit_of_num_IMP_loop_body_def)
+    apply(simp only: prefix_simps)
+    apply(vcg_time nth_bit_of_num_IMP_vars)
+    by (fastforce_sorted_premises simp: Let_def nth_bit_of_num_complete_time_simps)
   done
-
-
-
 
 
 subsection \<open>nth_bit_tail\<close>
@@ -713,8 +582,7 @@ lemma nth_bit_tail_imp_correct:
   apply (induction s rule: nth_bit_tail_imp.induct)
   apply (subst nth_bit_tail_imp.simps)
   apply (subst nth_bit_tail'.simps)
-  apply (simp del: nth_bit_tail.simps add: nth_bit_tail_imp_subprogram_simps Let_def)
-  done
+  by (simp del: nth_bit_tail.simps add: nth_bit_tail_imp_subprogram_simps Let_def)
 
 definition "nth_bit_tail_state_upd_time t s \<equiv>
   let
@@ -798,7 +666,7 @@ lemma nth_bit_tail_imp_time_acc_2:
 lemma nth_bit_tail_imp_time_acc_3:
   "(nth_bit_tail_imp_time (a + b) s) = a + (nth_bit_tail_imp_time b s)"
   by (induction a arbitrary: b s)
-      (simp add: nth_bit_tail_imp_time_acc)+
+    (simp add: nth_bit_tail_imp_time_acc)+
 
 abbreviation "nth_bit_tail_while_cond \<equiv> ''condition''"
 
@@ -864,40 +732,37 @@ lemmas nth_bit_tail_complete_simps =
 
 lemma nth_bit_tail_IMP_Minus_correct_function:
   "(invoke_subprogram p nth_bit_tail_IMP_Minus, s) \<Rightarrow>\<^bsup>t\<^esup> s' \<Longrightarrow>
-     s' (add_prefix p nth_bit_tail_ret_str)
-      = nth_bit_tail_ret
-          (nth_bit_tail_imp (nth_bit_tail_imp_to_HOL_state p s))"
+     s' (add_prefix p nth_bit_tail_ret_str) =
+      nth_bit_tail_ret (nth_bit_tail_imp (nth_bit_tail_imp_to_HOL_state p s))"
   apply(induction "nth_bit_tail_imp_to_HOL_state p s" arbitrary: s s' t
       rule: nth_bit_tail_imp.induct)
   apply(subst nth_bit_tail_imp.simps)
   apply(simp only: nth_bit_tail_IMP_Minus_def prefix_simps)
-  apply(erule Seq_tE)+
-  apply(erule While_tE)
-   apply(simp only: nth_bit_tail_IMP_subprogram_simps prefix_simps)
-   apply(erule Seq_tE)+
-   apply(fastforce simp: nth_bit_tail_IMP_subprogram_simps
-      nth_bit_tail_imp_subprogram_simps
-      nth_bit_tail_state_translators)
-  apply(erule Seq_tE)+
-  apply(dest_com_gen)
+  apply(vcg nth_bit_tail_IMP_vars)
 
   subgoal
-    apply(simp only: nth_bit_tail_IMP_init_while_cond_def prefix_simps)
-    by(fastforce simp add: nth_bit_tail_complete_simps)
+    apply(subst (asm) (3) nth_bit_tail_IMP_init_while_cond_def)
+    apply(subst (asm) (2) nth_bit_tail_IMP_after_loop_def)
+    apply(simp only: prefix_simps)
+    apply(vcg nth_bit_tail_IMP_vars)
+    by (fastforce simp: nth_bit_tail_complete_simps)
 
   subgoal
-    apply(simp only: nth_bit_tail_IMP_init_while_cond_def nth_bit_tail_IMP_loop_body_def
-        prefix_simps)
-    apply(erule Seq_tE)+
-    apply (simp add: nth_bit_tail_complete_simps Let_def)
-    by force
+    apply(subst (asm) (1) nth_bit_tail_IMP_init_while_cond_def)
+    apply(simp only: prefix_simps)
+    by (fastforce simp add: nth_bit_tail_complete_simps)
 
   subgoal
-    apply(simp only: nth_bit_tail_IMP_init_while_cond_def nth_bit_tail_IMP_loop_body_def
-        prefix_simps)
-    apply(erule Seq_tE)+
-    apply (simp add: nth_bit_tail_complete_simps Let_def)
-    by force
+    apply(subst (asm) nth_bit_tail_IMP_init_while_cond_def)
+    apply(subst (asm) nth_bit_tail_IMP_loop_body_def)
+    apply(simp only: prefix_simps)
+    by (fastforce simp add: Let_def nth_bit_tail_complete_simps)
+
+  subgoal
+    apply(subst (asm) (1) nth_bit_tail_IMP_init_while_cond_def)
+    apply(subst (asm) (1) nth_bit_tail_IMP_loop_body_def)
+    apply(simp only: prefix_simps)
+    by (fastforce simp add: Let_def nth_bit_tail_complete_simps)
   done
 
 lemma nth_bit_tail_IMP_Minus_correct_effects:
@@ -910,7 +775,6 @@ lemma nth_bit_tail_IMP_Minus_correct_effects:
 lemmas nth_bit_tail_complete_time_simps =
   nth_bit_tail_imp_subprogram_time_simps
   nth_bit_tail_IMP_subprogram_simps
-  nth_bit_tail_imp_time_acc
   nth_bit_tail_imp_time_acc_2
   nth_bit_tail_imp_time_acc_3
   nth_bit_tail_state_translators
@@ -923,37 +787,35 @@ lemma nth_bit_tail_IMP_Minus_correct_time:
   apply(subst nth_bit_tail_imp_time.simps)
   apply(simp only: nth_bit_tail_IMP_Minus_def prefix_simps)
 
-  apply(erule Seq_tE)+
-  apply(erule While_tE_time)
-  subgoal
-    apply(simp only: nth_bit_tail_IMP_subprogram_simps prefix_simps)
-    apply(erule Seq_tE)+
-    by (force simp: nth_bit_tail_IMP_subprogram_simps
-        nth_bit_tail_imp_subprogram_time_simps nth_bit_tail_state_translators)
+  apply(vcg_time nth_bit_tail_IMP_vars)
 
-  apply(erule Seq_tE)+
+  subgoal
+    apply(subst (asm) (3) nth_bit_tail_IMP_init_while_cond_def)
+    apply(subst (asm) (2) nth_bit_tail_IMP_after_loop_def)
+    apply(simp only: prefix_simps)
+    apply(vcg_time nth_bit_tail_IMP_vars)
+    by (force simp add: nth_bit_tail_IMP_subprogram_simps nth_bit_tail_imp_subprogram_time_simps
+        nth_bit_tail_state_translators)
+
   apply(simp add: add.assoc)
-  apply(dest_com_gen_time)
+  apply(vcg_time nth_bit_tail_IMP_vars)
 
   subgoal
-    apply(simp only: nth_bit_tail_IMP_init_while_cond_def prefix_simps)
-    by(fastforce simp add: nth_bit_tail_complete_simps)
+    apply(subst (asm) (1) nth_bit_tail_IMP_init_while_cond_def)
+    apply(simp only: prefix_simps)
+    by (fastforce simp add: nth_bit_tail_complete_simps)
 
   subgoal
-    apply(subst (asm) nth_bit_tail_IMP_init_while_cond_def)
-    apply(simp only:
-        nth_bit_tail_IMP_loop_body_def prefix_simps)
-    apply(erule Seq_tE)+
-    by (simp only: nth_bit_tail_imp_subprogram_time_simps
-        nth_bit_tail_state_translators Let_def, force)
+    apply(subst (asm) (1) nth_bit_tail_IMP_init_while_cond_def)
+    apply(subst (asm) (1) nth_bit_tail_IMP_loop_body_def)
+    apply(simp only: prefix_simps)
+    by (fastforce simp add: Let_def nth_bit_tail_complete_time_simps)
 
   subgoal
-    apply(simp only: prefix_simps nth_bit_tail_IMP_init_while_cond_def
-        nth_bit_tail_IMP_loop_body_def)
-    apply(erule Seq_tE)+
-    apply(simp only: nth_bit_tail_complete_time_simps Let_def)
-    by force
-
+    apply(subst (asm) (1) nth_bit_tail_IMP_init_while_cond_def)
+    apply(subst (asm) (1) nth_bit_tail_IMP_loop_body_def)
+    apply(simp only: prefix_simps)
+    by (fastforce simp add: Let_def nth_bit_tail_complete_time_simps)
   done
 
 lemma nth_bit_tail_IMP_Minus_correct:
@@ -968,5 +830,5 @@ lemma nth_bit_tail_IMP_Minus_correct:
   using nth_bit_tail_IMP_Minus_correct_function
   by (auto simp: nth_bit_tail_IMP_Minus_correct_time)
     (meson nth_bit_tail_IMP_Minus_correct_effects set_mono_prefix)
-  
-end 
+
+end
