Cook_Levin/IMP-_To_SAS+/IMP-_To_IMP--/Utilities.thy
@@ -1,0 +1,157 @@
+theory Utilities
+  imports
+    IMP_Minus.Call_By_Prefixes
+    IMP_Minus.Com
+begin
+
+
+lemma Seq_E:
+  "\<lbrakk>(c1;; c2, s1) \<Rightarrow>\<^bsup> p \<^esup> s3; \<And>x s2 y. \<lbrakk>(c1, s1) \<Rightarrow>\<^bsup> x \<^esup> s2; (c2, s2) \<Rightarrow>\<^bsup> y \<^esup> s3\<rbrakk> \<Longrightarrow> P\<rbrakk> \<Longrightarrow> P"
+  by blast
+thm If_tE[where ?x=y]
+
+lemma If_E:
+  "\<lbrakk>(IF b\<noteq>0 THEN c1 ELSE c2, s) \<Rightarrow>\<^bsup> y \<^esup> t; \<And>x. \<lbrakk>0 < s b; (c1, s) \<Rightarrow>\<^bsup> x \<^esup> t\<rbrakk> \<Longrightarrow> P;
+    \<And>x. \<lbrakk>s b = 0; (c2, s) \<Rightarrow>\<^bsup> x \<^esup> t\<rbrakk> \<Longrightarrow> P\<rbrakk>
+  \<Longrightarrow> P"
+  by blast
+
+
+method fastforce_sorted_premises uses simp =
+  (match premises in
+    var_doesnt_change[thin]: "\<And>x. x \<in>  _ \<Longrightarrow> _ (_ x) = _ (_ x)"(multi)
+    \<Rightarrow> \<open>match premises in
+        subroutine_results[thin]: "_ (add_prefix (add_prefix p _) _) = _" (multi) for p
+          \<Rightarrow> \<open>match premises in
+            assignments[thin]: "((add_prefix p1 _) ::= _, _) \<Rightarrow>\<^bsup> _ \<^esup> _" (multi) for p1
+              \<Rightarrow> \<open>match premises in
+                while_cond[thin]: "_ < _ (add_prefix p2 _)" (multi) for p2
+                  \<Rightarrow> \<open>match premises in
+                    invoke[thin]: "(invoke_subprogram p3 _, _) \<Rightarrow>\<^bsup> _ \<^esup> _" (multi) for p3
+                      \<Rightarrow> \<open>match premises in
+                        remaining[thin]: "_" (multi)
+                          \<Rightarrow> \<open>insert var_doesnt_change subroutine_results while_cond invoke,
+                             (fastforce simp add: assignments[THEN AssignD, simplified]
+                                remaining simp)\<close>\<close>\<close>\<close>\<close>\<close>)
+
+method force_sorted_premises uses simp =
+  (match premises in
+    var_doesnt_change[thin]: "\<And>x. x \<in>  _ \<Longrightarrow> _ (_ x) = _ (_ x)"(multi)
+    \<Rightarrow> \<open>match premises in
+        subroutine_results[thin]: "_ (add_prefix (add_prefix p _) _) = _" (multi) for p
+          \<Rightarrow> \<open>match premises in
+            assignments[thin]: "((add_prefix p1 _) ::= _, _) \<Rightarrow>\<^bsup> _ \<^esup> _" (multi) for p1
+              \<Rightarrow> \<open>match premises in
+                while_cond[thin]: "_ < _ (add_prefix p2 _)" (multi) for p2
+                  \<Rightarrow> \<open>match premises in
+                    invoke[thin]: "(invoke_subprogram p3 _, _) \<Rightarrow>\<^bsup> _ \<^esup> _" (multi) for p3
+                      \<Rightarrow> \<open>match premises in
+                        remaining[thin]: "_" (multi)
+                          \<Rightarrow> \<open>insert var_doesnt_change subroutine_results while_cond invoke,
+                             (force simp add: assignments[THEN AssignD, simplified]
+                                remaining simp)\<close>\<close>\<close>\<close>\<close>\<close>)
+
+method sort_premises =
+  (match premises in
+    var_doesnt_change[thin]: "\<And>x. x \<in>  _ \<Longrightarrow> _ (_ x) = _ (_ x)"(multi)
+    \<Rightarrow> \<open>match premises in
+        subroutine_results[thin]: "_ (add_prefix (add_prefix p _) _) = _" (multi) for p
+          \<Rightarrow> \<open>match premises in
+            assignments[thin]: "((add_prefix p1 _) ::= _, _) \<Rightarrow>\<^bsup> _ \<^esup> _" (multi) for p1
+              \<Rightarrow> \<open>match premises in
+                while_cond[thin]: "_ < _ (add_prefix p2 _)" (multi) for p2
+                  \<Rightarrow> \<open>match premises in
+                    invoke[thin]: "(invoke_subprogram p3 _, _) \<Rightarrow>\<^bsup> _ \<^esup> _" (multi) for p3
+                      \<Rightarrow> \<open>match premises in
+                    remaining[thin]: "_" (multi)
+                      \<Rightarrow> \<open>insert var_doesnt_change subroutine_results while_cond invoke assignments
+                          remaining\<close>\<close>\<close>\<close>\<close>\<close>)
+
+
+definition "While' = Com.com.While"
+
+notation While' ("(WHILEdummy _/\<noteq>0 DO _)"  [0, 61] 61)
+
+lemma While_E_dummy:
+  "\<lbrakk>(WHILE b\<noteq>0 DO c, s) \<Rightarrow>\<^bsup> x \<^esup> t;
+    \<lbrakk>t = s; s b = 0\<rbrakk> \<Longrightarrow> P;
+    \<And>x' s2 y. \<lbrakk>0 < s b; (c, s) \<Rightarrow>\<^bsup> x' \<^esup> s2;
+               (WHILEdummy b\<noteq>0 DO c, s2) \<Rightarrow>\<^bsup> y \<^esup> t\<rbrakk> \<Longrightarrow> P\<rbrakk>
+  \<Longrightarrow> P"
+  by (auto simp: While'_def)
+
+lemma While_tE_dummy:
+  "\<lbrakk>(WHILE b\<noteq>0 DO c, s) \<Rightarrow>\<^bsup> x \<^esup> t;
+  \<lbrakk>x = Suc (Suc 0); t = s; s b = 0\<rbrakk> \<Longrightarrow> P;
+  \<And>x' s2 y. \<lbrakk>0 < s b; (c, s) \<Rightarrow>\<^bsup> x' \<^esup> s2;
+             (WHILEdummy b\<noteq>0 DO c, s2) \<Rightarrow>\<^bsup> y \<^esup> t; x = Suc (x' + y)\<rbrakk> \<Longrightarrow> P\<rbrakk> \<Longrightarrow> P"
+  by (auto simp: While'_def)
+
+method while_step = (erule While_E_dummy, print_fact While_E_dummy)
+method while_step_time = (erule While_tE_dummy, print_fact While_tE_dummy)
+method seqt_step = (erule Seq_tE, print_fact Seq_tE)
+method seq_step = (erule Seq_E, print_fact Seq_E)
+method ift_step = (erule If_tE, print_fact If_tE)
+method if_step = (erule If_E, print_fact If_E)
+method assign_step = (drule AssignD, elim conjE, print_fact AssignD)
+
+definition "dest_com_gen = 0"
+
+lemma dest_com_gen: "dest_com_gen = dest_com_gen"
+  by simp
+
+named_theorems functional_correctness
+
+method subroutine_step for vars::"char list set" =
+  (match premises in foo[thin]:
+    "(invoke_subprogram (add_prefix _ _) subprog, _) \<Rightarrow>\<^bsup> _ \<^esup> _" for subprog
+    \<Rightarrow> \<open>match functional_correctness in invokeE[thin]:
+          "\<And>(vars:: char list set). \<lbrakk>(invoke_subprogram (add_prefix _ _) subprog, _) \<Rightarrow>\<^bsup> _ \<^esup> _;
+           _; _\<rbrakk> \<Longrightarrow> ?P"
+            \<Rightarrow> \<open>insert foo; elim invokeE[where ?vars=vars]\<close>\<close>,
+    match premises in prem: "_ \<in> vars" \<Rightarrow> \<open>insert prem, fastforce\<close>)
+
+definition "subroutine_step = 0"
+
+lemma subroutine_step: "subroutine_step = subroutine_step"
+  by auto
+
+method dest_com_gen' =
+  (erule compose_programs_1[where ?c2.0 = "(While' _ _)"], assumption,
+    erule compose_programs_2[where ?c1.0 = "(_;; While' _ _)"], assumption,
+    (match premises in a[thin]:
+      "(init_while_cond;;
+        WHILEdummy _ \<noteq>0 DO (
+          loop_body;;
+          init_while_cond);;
+        after_loop, _) \<Rightarrow>\<^bsup>_\<^esup> _" for init_while_cond loop_body after_loop  \<Rightarrow>
+      \<open>match premises in b[thin]: "\<lbrakk>loop_cond; state_upd; _\<rbrakk> \<Longrightarrow> P"
+        for loop_cond state_upd P \<Rightarrow> \<open>subst b[OF _ _ a[unfolded While'_def]]\<close>\<close>))
+
+method dest_com_gen_time' =
+  (erule compose_programs_1[where ?c2.0 = "(While' _ _)"], assumption,
+    erule compose_programs_2[where ?c1.0 = "(_;; While' _ _)"], assumption,
+    (match premises
+      in a[thin]:
+      "(init_while_cond;;
+                WHILEdummy _ \<noteq>0 DO (loop_body;; init_while_cond);;
+                after_loop, _) \<Rightarrow>\<^bsup>_\<^esup> _"
+    for init_while_cond loop_body after_loop  \<Rightarrow>
+      \<open>match premises in b[thin]: "\<lbrakk>loop_cond; state_upd; _\<rbrakk> \<Longrightarrow> P"
+       for loop_cond state_upd P \<Rightarrow> \<open>subst b[OF _ _ a[unfolded While'_def], simplified add.assoc]\<close>\<close>))
+
+method vcg for vars::"char list set" =
+  (((subroutine_step vars, print_fact subroutine_step); (vcg vars)?) |
+    (while_step ; (vcg vars)?) |
+    ((dest_com_gen', print_fact dest_com_gen) ; (vcg vars)?) |
+    (if_step ; (vcg vars)?) |
+    (seq_step ; (vcg vars)?))
+
+method vcg_time for vars::"char list set" =
+  (((subroutine_step vars, print_fact subroutine_step); (vcg_time vars)?) |
+    (while_step_time; (vcg_time vars)?) |
+    ((dest_com_gen_time', print_fact dest_com_gen); (vcg_time vars)?) |
+    (ift_step; (vcg_time vars)?) |
+    (seqt_step; (vcg_time vars)?))
+
+end
